\documentclass[20pt,a4paper]{extarticle}
\usepackage[a4paper,margin=6mm]{geometry}
\usepackage{amsmath}
\usepackage{hyperref}

\begin{document}
 Solution for Problem J369 \\
 After removing square roots from both sides of the original equation  we obtain\\
 \begin{equation}\label{eq:1}
  x^{6}+4x^{5}+4x^{4}-2x^{3}-4x^{2}+1=0. 
 \end{equation}
 
 $\Rightarrow  (x+1)^{2}(x^{4}+2x^{3}-x^{2}-2x+1)=0$ \\

 Thus  $\ref{eq:1}$  has a double root $=-1$  , but $-1$ is not the root of original equation
 hence they must be discarded.\\
 Dividing  \ref{eq:1}  by $(x+1)^{2}$ we obtain  
 \begin{equation}\label{eq:2}
  x^{4}+2x^{3}-x^{2}-2x+1=0
 \end{equation}
 
 
 $ \Rightarrow  (x-1)(x)(x+1)(x+2)=-1 \Rightarrow  (x^{2}+x-1)^{2}=0
 \Rightarrow  x=\frac{-1\pm \sqrt{5}}{2} $. \\
Plugging these roots to original equation , we get that  $ x= \frac{ \sqrt{5}-1}{2}$ is the only solution of the given equation.
  

\end{document}