\documentclass[20pt,a4paper]{extarticle}
\usepackage[a4paper,margin=6mm]{geometry}
\usepackage{amsmath}
\usepackage{hyperref}

\begin{document}
 
 Arpon Basu\\
 AECS-4 , Mumbai-400094\\
 
 Solution for Problem J371 \\
 
 
 After manipulating the expression $ {n+3 \choose 2} + 6{n+4 \choose 4} + 90{n+5 \choose 6}$ we obtain \\
 

 $ {n+3 \choose 2} + 6{n+4 \choose 4} + 90{n+5 \choose 6}=\frac{n^{2}+5n+6}{2} (1+ \frac{(n^{2}+5n+4)(n^{2}+5n+2)}{4})$ \\
 
 
 let $a=(n^{2}+5n+2).$\\
 
 $ {n+3 \choose 2} + 6{n+4 \choose 4} + 90{n+5 \choose 6}=\frac{a+4}{2} (4+ \frac{(a)(a+2)}{4})$ \\
 
 After manipulation we obtain 
 
 $ {n+3 \choose 2} + 6{n+4 \choose 4} + 90{n+5 \choose 6}=\frac{a+4}{2} (4+ \frac{(a)(a+2)}{4})=(\frac{a}{2}+1)^{3}+(1)^3$ \\
 
  For even $n$, $a=n(n+5)+2$ is even. For odd $n$, $(n+5)$ is even making $a$ even.Thus for all integer $n$,$\frac{a}{2}$ is an integer.\\
  So $ {n+3 \choose 2} + 6{n+4 \choose 4} + 90{n+5 \choose 6}=(\frac{a}{2}+1)^{3}+(1)^3$ is sum of two perfect cubes. 
 
 

\end{document}