\documentclass[10pt,a4paper]{extarticle}
\usepackage[a4paper,margin=6mm]{geometry}
\usepackage{amsmath}


\begin{document}
Arpon Basu, School: AECS-4 , Mumbai-400094\\
Solution for Problem J373 \\
$$a^{2}+b^{2}+2=a^{2}+b^{2}+1+1=a^{2}+1+b^{2}+1\geq \frac{(a+1)^{2}}{2}+\frac{(b+1)^{2}}{2}\geq 2\sqrt{\frac{(a+1)^{2}(b+1)^{2}}{4}}=(a+1)(b+1)$$ whereby the inequalities are true by direct application of the AM-GM inequality.\\
Therefore we get that:
$$(a^{2}+b^{2}+2)(b^{2}+c^{2}+2)(c^{2}+a^{2}+2)\geq (a+1)(b+1)(b+1)(c+1)(c+1)(a+1)=(a+1)^{2}(b+1)^{2}(c+1)^{2}$$\\
Since $a^{2}+1\geq \frac{(a+1)^{2}}{2}$ is true for all $a\geq -1$,we conclude that the inequality holds for all real $a,b,c\geq -1$\\

\end{document}