\documentclass[10pt,a4paper]{extarticle}
\usepackage[a4paper,margin=6mm]{geometry}
\usepackage{amsmath}


\begin{document}
 
 Arpon Basu, School: AECS-4 , Mumbai-400094\\
 
 Solution for Problem J375 \\
 
 $x^{1/3}+y^{1/3}=\frac{1}{2}+(x+y+\frac{1}{4})^{1/2}$\\
$\Rightarrow x^{1/3}+y^{1/3}=\frac{1}{2}+\frac{(4x+4y+1)^{1/2}}{2}$\\
Now,let $x^{1/3}=a$ and $y^{1/3}=b$.Thus,\\
$2(a+b)-1=(1+4a^{3}+4b^{3})^{\frac{1}{2}}$\\
$\Rightarrow 4(a+b)^{2}+1-4(a+b)=1+4a^{3}+4b^{3}$\\
$\Rightarrow (a+b)^{2}-(a+b)=a^{3}+b^{3}=(a+b)(a^{2}-ab+b^{2})$.\\
$\Rightarrow (a+b)(a+b-1)=(a+b)(a^{2}-ab+b^{2})$.\\
$(a+b)\neq 0$ for if $a+b=0$ then LHS is 0 while RHS is 1 \\
So factoring out the $a+b$ and canceling  we get:-\\
$\Rightarrow a+b-1=a^{2}-ab+b^{2} $.\\
$\Rightarrow a^{2}-(b+1)a+b^{2}-b+1=0$. Solving this equation by treating it as a quadratic in $a$,we get,\\
$\Rightarrow a=\frac{b+1\pm \sqrt{-3b^{2}+6b-3}}{2}$\\
$\Rightarrow a=\frac{b+1\pm \sqrt{-3(b-1)^{2}}}{2}$\\
Since $-3(b-1)^{2}\leq 0$,and since $a$ has to be a real number,this forces \\
$-3(b-1)^{2}=0\Rightarrow b=1\Rightarrow a=1$ \\
$ \Rightarrow x=a^{3}=1$,$y=b^{3}=1 $\\
Thus $(1,1)$ is the \textit{only real solutions} of the given equation.\\
 
 
\end{document}