\documentclass[a4paper,10pt]{article}
\usepackage[utf8x]{inputenc}
\usepackage{amsmath}
\usepackage{amssymb}

\begin{document}
\begin{center}


Arpon Basu,School: AECS-4,Mumbai-400094

Solution for problem J439
\end{center}
\textbf{We claim that} $\mathbf{ (x,y,z) = (1,1,1),(-1,-1,-1)}$ \textbf{are the only solutions.}\\


We subtract the third equation from sum of first two equations.


\begin{equation*}
\begin{split}
(2x^2-3xy+2y^2)+(y^2-3xy+4y^2)-(z^2+3zx-x^2)&=1+2-3 \\
                                            &=0 \\
\Rightarrow 3(x^2+y^2+z^2-xy-yz-zx)=0 \\
\Rightarrow (x-y)^2+(y-z)^2+(z-x)^2=0 \\
\therefore (x-y)=(y-z)=(z-x)=0 \\
\Rightarrow x=y=z
\end{split}
\end{equation*}

Putting $x=y=z$ in all the three given equation we obtain $x^2=y^2=z^2=1$\\
$\mathbf{\therefore (x,y,z) = (1,1,1),(-1,-1,-1)}$ \textbf{are the only solutions.} \\
Plugging these solutions in the three given equations we verify that they work.


\end{document}
