\documentclass[a4paper,10pt]{article}
\usepackage[utf8x]{inputenc}
\usepackage{amsmath}
\usepackage{amssymb}

\begin{document}
\begin{center}


Arpon Basu,School: AECS-4,Mumbai-400094

Solution for problem J442
\end{center}

We use barrycentric coordinates.
let $$A:(1,0,0) $$
    $$B:(0,1,0) $$
    $$C:(0,0,1) $$

Where $\triangle ABC$ is our reference triangle.

$$ \therefore \hspace{10pt} O:(\frac{1}{3},\frac{1}{3},\frac{1}{3}) $$
where $O$ is the centre of triangle.\\
Let $M$ be $(1-t,t,0)$ where $t \in \mathbb{R}$. We note that $M \in \overleftrightarrow{AB}$ \\
$ \because M,O,N $ are collinear , 

\begin{center}
 \begin{math}
 \begin{vmatrix}
  1-t & t & 0\\
  \frac{1}{3} & \frac{1}{3} & \frac{1}{3}\\
  X_{N} & Y_{N} & Z_{N}
\end{vmatrix}=0
\end{math}
\end{center}



$ \because N \in \overleftrightarrow{AC} , Y_{N}=0 $  solving for $ X_{N} , Z_{N}$ we get $N:(2t-1:0:t)$ \\

$ \therefore \overleftrightarrow{BN}$ is represented by 

\begin{center}
\begin{math}
 \begin{vmatrix}
  0 & 1 & 0\\
  (2t-1) & 0 & t \\
 x & y & z
\end{vmatrix}=0 
\end{math}
\vspace{5pt} \\
\begin{math}
\Rightarrow tx+(1-2t)z=0
\end{math}
\end{center}



$ \overleftrightarrow{CM}$ is represented by 

\begin{center}
\begin{math}
 \begin{vmatrix}
  0 & 0 & 1\\
  (1-t) & t & 0 \\
 x & y & z
\end{vmatrix}=0 
\end{math}
\vspace{5pt} \\
\begin{math}
\Rightarrow tx+(1-t)y=0
\end{math}
\end{center}


\begin{equation}
\begin{split}
  \therefore k &=\overleftrightarrow{BN} \cap \overleftrightarrow{CM} \\
               &= \big((1-t)(2t-1):t(2t-1):t(1-t)\big)
\end{split}
\end{equation}


\begin{center}
\begin{math}
 \therefore \overleftrightarrow{AK}:
\begin{vmatrix}
  1 & 0 & 0\\
  (1-t)(2t-1) & t(2t-1) & t(1-t) \\
   x & y & z
\end{vmatrix}=0 
\end{math}
\vspace{5pt} \\
\begin{math}
\Rightarrow (1-t)y+(1-2t)z=0
\end{math}
\end{center}


Also
\begin{center}
\begin{math}
 \overleftrightarrow{BO}:
\begin{vmatrix}
  0 & 1 & 0\\
  \frac{1}{3} & \frac{1}{3} & \frac{1}{3} \\
   x & y & z
\end{vmatrix}=0 
\end{math}
\vspace{5pt} \\
\begin{math}
\Rightarrow (x-z)=0
\end{math}
\end{center}



\begin{equation}
\begin{split}
  \therefore P &=\overleftrightarrow{AK} \cap \overleftrightarrow{BO} \\
             & = \big((1-t),(2t-1),(1-t)\big)
\end{split}
\end{equation}


$\therefore $ the displacement vectors are 


\begin{center}
\begin{math}
 \overrightarrow{MB}=\big((1-t),(t-1),0\big)
\end{math}
\end{center}


\begin{center}
\begin{math}
 \overrightarrow{MP}=\big(0,(1-t),(t-1)\big)
\end{math}
\end{center}

\begin{center}
\begin{equation}
\begin{split}
&\therefore |\overrightarrow{MB}|^2 = -a^2yz - b^2zx -c^2xy = c^2(1-t)^2  \\
&\therefore |\overrightarrow{MP}|^2 = -a^2(1-t)(t-1)=a^2(1-t)^2 
\end{split}
\end{equation}
\end{center}

$\because \triangle ABC$ is equilateral $\therefore a=c \Rightarrow MB=MP $ \\

\textbf{Hence Proved}

Note: Our proof works exactly even if only  $BC=A$ as the centroid
 
\end{document}
