\documentclass[a4paper,10pt]{article}
\usepackage[utf8]{inputenc}
\usepackage{amssymb}
\usepackage{amsmath}
%opening
\title{}
\author{}

\begin{document}


\begin{center}


Arpon Basu,School: AECS-4,Mumbai-400094

Solution for problem O433
\end{center}


Given 
\begin{equation} \label{eq1}
 3qr=s^2 -s+1
\end{equation}




Multiplying both side of equation 1 by $s$ we obtain

\begin{equation} 
\begin{split}
(3qr)s & = (s^2 -s+1)s \\
 & = s^3-s^2+s
\end{split}
\end{equation}


\begin{equation} 
\begin{split}
\therefore q^3+r^3-s^3+3qrs & = q^3+r^3-s^3+s^3-s^2+s  \\
 & = q^3+r^3-(s^2-s)
\end{split}
\end{equation}


From equation 1 we obtain $$(s^2 -s)=3qr-1 $$ \\
Replacing value of $(s^2 -s)$ in quation 3 we obtain


\begin{equation} \label{}
\begin{split}
 q^3+r^3-s^3+3qrs &= q^3+r^3-(s^2-s) \\
 & = q^3+r^3+1 - 3qr \\
 & =q^3+r^3+1^3 - 3qr(1)\\
 & =(q+r+1)(q^2+r^2+1-qr-q-r)
\end{split}
\end{equation}
 
 
$$\therefore (q+r+1) \mid q^3+r^3-s^3+3qrs $$

Hence Proved     

\end{document}



 