\documentclass[a4paper,10pt]{article}
\usepackage[utf8x]{inputenc}
\usepackage{amsmath}
\usepackage{amssymb}

\begin{document}
\begin{center}


Arpon Basu,School: AECS-4,Mumbai-400094

Solution for problem O436
\end{center}


Let $a=x+y$,$b=y+z$,$c=z+x$ where $x,y,z \in R_{\ge 0}$. Then $a,b,c$ follow the triangle inequality .\\
Also  
$$ s=\frac{a+b+c}{2}=\frac{(x+y)+(y+z)+(z+x)}{2}=x+y+z$$
$$ \sin \frac{A}{2}=\sqrt{\frac{(s-b)(s-c)}{bc}}=\sqrt{\frac{xy}{(y+z)(z+x)}}$$
$$  \sum_{cyclic}\frac{a^2}{\sin(\frac{A}{2})} = \sum_{cyclic} \frac{(x+y)^2}{\sqrt{\frac{xy}{(y+z)(z+x)}}}  $$

$$ =\sqrt{\frac{(x+y)(y+z)(z+x)}{xyz}} \sum_{cyclic} \sqrt{x(y+z)^3}  $$

We now observe that the inequality is homogeneous, so we put $x+y+z=1$

We get 

\begin{align*}
 \sqrt{\frac{(1-x)(1-y)(1-z)}{xyz}}\sum_{cyclic}\sqrt{x(1-x)^3} \ge 0 &&\text{(To be proved)}
\end{align*}

Applyying AM-GM inequality 
$$ \sum_{cyclic}\sqrt{x(1-x)^3} \ge 3 \sqrt[3]{\prod_{cyclic}}\sqrt{x(1-x)^3}  $$
$$ \prod_{cyclic} \sqrt{\frac{1-x}{x}} \sum_{cyclic} \sqrt{x(1-x)^3} \ge 3 \prod_{cyclic} \frac{(1-x)}{\sqrt[3]{x}} $$

Thus if we can prove that 

\begin{align*}
 3\prod_{cyclic}\frac{(1-x)}{\sqrt[3]{x}} \ge \frac{8}{3} &&\text{then we are done} \\
 \Rightarrow \prod_{cyclic}\frac{(1-x)}{\sqrt[3]{x}} \ge \frac{8}{9}
\end{align*}



We define 
 
\begin{align*}
    \mathcal{L}(x,y,z,\lambda)=\underbrace{\prod_{cyclic}\frac{(1-x)}{\sqrt[3]{x}}}_\text{function to be optimized} -\lambda \underbrace{ (x+y+z-1)}_\text{constraints} &&\text{for applying Lagrange multiplier}   
\end{align*}


\begin{align*}
 &\Rightarrow \nabla\mathcal{L}=0 \\
 &\therefore \lambda = -x^{-\frac{4}{3}} \frac{(1-y)(1-z)}{\sqrt[3]{yz}} &\text{(cyclic equation for $y,z$ hold)} \\
 &\therefore -x^{-\frac{4}{3}} \frac{(1-y)(1-z)}{\sqrt[3]{yz}}=-y^{-\frac{4}{3}} \frac{(1-z)(1-x)}{\sqrt[3]{zx}}=-z^{-\frac{4}{3}} \frac{(1-x)(1-y)}{\sqrt[3]{xy}} \\
 &\Rightarrow \frac{1-x}{x}=\frac{1-y}{y}=\frac{1-z}{z} \\
 &\Rightarrow x=y=z \\
 &\Rightarrow x=y=z=\frac{1}{3} \\
\end{align*}
Evaluating $$\prod_{cyclic}\frac{(1-x)}{\sqrt[3]{x}}$$ for $(\frac{1}{3},\frac{1}{3},\frac{1}{3})$, we get the value $\frac{8}{9}$.\\ 
Putting any other value $(x,y,z)$ subject to $x+y+z=1$ makes $$\prod_{cyclic}\frac{(1-x)}{\sqrt[3]{x}}$$ greater than  $\frac{8}{9}$, implying  $\frac{8}{9}$
is the global minima on $x+y+z=1$.\\
Thus $\prod \frac{(1-x)}{\sqrt[3]{x}} \ge \frac{8}{9}$ hence our original inequality is proved.


\end{document}
