\documentclass[10pt,a4paper]{extarticle}
\usepackage[a4paper,margin=6mm]{geometry}
\usepackage{amsmath}


\begin{document}
Arpon Basu, School: AECS-4 , Mumbai-400094\\
Solution for Problem O387 \\
We check the modulo 7 of the expression $3^{(6n-3)} + 3^{(3n-1)} + 1 $. \\
$3^{(6n-3)} = 3^{3(2n-1)}=27^{(2n-1)} \equiv (-1)^{(2n-1)} \equiv -1 (\textrm{mod}\ 7) $ \\
$3^{(3n-1)} =(9)(3^{3n-3)})=(9)27^{(n-1)} \equiv (9)(-1)^{(n-1)} \equiv (2)(-1)^{(n-1)} (\textrm{mod}\ 7) $ \\
$3^{(6n-3)} + 3^{(3n-1)} + 1  \equiv (-1+(2)(-1)^{(n-1)}+1) (\textrm{mod}\ 7) \equiv (2)(-1)^{(n-1)} (\textrm{mod}\ 7) \equiv 2,5 (\textrm{mod}\ 7) $ \\
But cubic residude modulo 7 is ${0,1,6}$. Hence given expression can't be a perfect cube.
 
\end{document}