\documentclass[10pt,a4paper]{extarticle}
\usepackage[a4paper,margin=6mm]{geometry}
\usepackage{amsmath}
\usepackage{amssymb}

\begin{document}
\begin{center}


Arpon Basu, School: AECS-4 , Mumbai-400094

Solution for problem O397
\end{center}

$$(x^3 -1)(y^3 -1)=3(x^2 + y^2 + 2)$$
$$\Leftrightarrow (x^3 y^3 - x^3 - y^3 +1-3x^2 y^2 + 6) = 0 $$
$$\Leftrightarrow (y^3 -1)x^3 -3y^2x^2 -(y^3+5)=0    $$
Now, if we consider $y$ is an integer constant, then we are basically searching for integer roots of this cubic polynomial in $x$An integer root is also a rational root
. Let $\frac{p}{q}$ be a root of this equation such that $(p,q)=1 , q \neq 0$ . Hence by rational root theorem 
$$ p  \mid (y^3 +5), q \mid (y^3 -1) $$. \\
Now $ \frac{p}{q} $ has to be an integer $ \Rightarrow q \mid p  $ \\
A divisor of $$(y^3 -1)$$ divides a divisor of $$(y^3 +5)$$ 
$ \Rightarrow$ there quotient divides $((y^3 -1),(y^3 +5))$. \\
Note that $$((y^3 -1),(y^3 +5))  \mid ((y^3 +5)-(y^3 -1)) \mid 6 $$
          $$((y^3 -1),(y^3 +5))  \mid 6$$
          $$ \Rightarrow   x=\frac{p}{q} = \pm 1 , \pm 2 \pm 3   $$ 
Checking for these values of $x$ we get that only \\
$x=1  \Rightarrow y^2 = -2 $ ( Impossible) \\
$x=-1 \Rightarrow 2y^3 + 3y^2+4 =0  \Rightarrow y=-2$ ( No integral root by Rational Root Theorem(RRT))\\
$x=2  \Rightarrow 7y^3 - 12y^2 -13 =0  $ ( No integral root by RRT) \\
$x=-2 \Rightarrow 3y^3 +4y^2 -1 =0  \Rightarrow y=-1$  \\
$x=3  \Rightarrow 26y^3 - 27y^2 -32 =0  $ ( No integral root by RRT) \\
$x=-3 \Rightarrow 28y^3 + 27y^2 -22 =0  $ ( No integral root by RRT) \\

Thus only roots are $(-1,-2)$ and $(-2,-1)$
          









\end{document}


