\documentclass[10pt,a4paper]{extarticle}
\usepackage[a4paper,margin=6mm]{geometry}
\usepackage{amsmath}
\usepackage{amssymb}

\begin{document}
\begin{center}


Arpon Basu, School: AECS-4 , Mumbai-400094

Solution for problem O402
\end{center}
We have to prove that 
$$\sin^{2}2A+\sin^{2}2B+\sin^{2}2C \ge 2\sqrt{3} \sin 2A \sin 2B \sin 2C$$
$$\Rightarrow 4 \sum_{sym} \sin^{2}A \cos^{2}A \ge 16\sqrt{3} \prod_{sym} \sin A \cos A $$
$$\Rightarrow  \sum_{sym} \sin^{2}A \cos^{2}A \ge 4\sqrt{3} \prod_{sym} \sin A \cos A $$

let $x=\sin A \cos A $ , $y=\sin B \cos B $ \& $z=\sin C \cos C $ then we need to prove that 
$$ x^{2}+y^{2}+z^{2} \ge 4\sqrt{3}xyz $$
If any of $ A, B ,C \in  [ \frac{\pi}{2} , \pi )  $ then $xyz \le 0 $ while $ x^{2}+y^{2}+z^{2} \ge 0 $ so inequality
is obviously true. \\ 
Thus we may assume $x,y,z > 0 $
It suffice to prove that 
$$ 3\sqrt[3]{x^{2}y^{2}z^{2}} \ge 4\sqrt{3} xyz$$
$$ \Leftrightarrow 3\sqrt[3]{(xyz)^{\frac{2}{3}}} \ge 4\sqrt{3} xyz$$
$$ \Leftrightarrow 3 \ge 4\sqrt{3} {(xyz)^{\frac{1}{3}}}$$
$$ \Leftrightarrow (\frac{\sqrt{3}}{4})^3 \ge xyz$$
$$ \Leftrightarrow (\frac{3\sqrt{3}}{64}) \ge xyz$$ \\
Now 
$$ xyz=\prod_{sym} \sin A \cos A = \prod_{sym} \sin A   \prod_{sym} \cos A$$  \\
Using the inequalities \\

$$\prod_{sym} \sin A \le \frac{3\sqrt{3}}{8} , \prod_{sym} \cos A \le \frac{1}{8} $$ we get \\
$$xyz \leq \frac{3\sqrt{3}}{8} \frac{1}{8} = \frac{3\sqrt{3}}{64}    $$      
  \textbf{QED}  \\
Equality occurs iff $$x=y=z \Rightarrow A=B=C=\frac{\pi}{3}$$










\end{document}


We know that $r_{a}=\frac{\bigtriangleup}{(s-a)}$ , $r_{b}=\frac{\bigtriangleup}{(s-b)}$ and $r_{c}=\frac{\bigtriangleup}{(s-c)}$ where $s$ is semi perimeter.\\
$$\therefore \frac{1}{r_{a}}=\frac{(s-a)}{\bigtriangleup} \Rightarrow \frac{1}{r_{a}h_{a}}=\frac{(s-a)}{{\bigtriangleup}{h_{a}}}$$ 
$$\therefore \sum{ \frac{1}{r_{a}h_{a}}}=\sum \frac{(s-a)}{{\bigtriangleup}{h_{a}}}=\frac{1}{\bigtriangleup}(\sum \frac{(s-a)}{h_{a}})$$
Now $$\frac{(s-a)}{{h_{a}}}=\frac{(\frac{b+c-a}{2})}{\frac{2 \bigtriangleup}{a}}=\frac{a(b+c-a)}{4 \bigtriangleup}$$ 
$$ \sum \frac{1}{r_{a}h_{a}}= \frac{1}{4{\bigtriangleup}^{2}} \sum  [(a)(b+c-a)]$$
$$= \frac{1}{4{\bigtriangleup}^{2}}[2(ab+bc+ca)-(a^{2}+b^{2}+c^{2})]$$
$$=\frac{1}{4{\bigtriangleup}^{2}}[a^{2}+b^{2}+c^{2}-(a-b)^{2}-(b-c)^{2} - (c-a)^{2}]$$ 
Now,by Hadwiger Finsler inequality , we know that 
$$a^{2}+b^{2}+c^{2}-(a-b)^{2} -(b-c)^{2} -(c-a)^{2} \geq 4\sqrt{3}\bigtriangleup$$ 
$\therefore  \sum \frac{1}{r_{a}h_{a}} \geq \frac{4\sqrt{3}\bigtriangleup}{4{\bigtriangleup}^{2}}=\frac{\sqrt{3}}{\bigtriangleup}$.(Proved)\\
 
Now $$\frac{1}{3r^{2}}=\frac{1}{3({\frac{\bigtriangleup}{s}})^{2}}=\frac{1}{3} (\frac{s}{\bigtriangleup})^2$$ 

We have to prove that $$ \frac{1}{3r^{2}} \geq \sum \frac{1}{r_{a}h_{a}}$$
$$  \Longleftrightarrow \frac{s^2}{3} \geq \frac{1}{4} \sum{[a(b+c-a)]}$$
$$ \Longleftrightarrow 4s^{2} \geq 3 \sum {[a(b+c-a)]} $$
$$\Longleftrightarrow (a+b+c)^{2} \geq 3[2(ab+bc+ca)-(a^2 + b^2 + c^2)]  $$

After algebraic manipulation we get $$ (a^2 +b^2 +c^2) \geq (ab+bc+ca) $$ But it is obviously true. Equalities occur, in both inequalities iff $$a=b=c $$ that is iff $\bigtriangleup$ABC is equilateral.