\documentclass[10pt,a4paper]{extarticle}
\usepackage[a4paper,margin=6mm]{geometry}
\usepackage{amsmath}


\begin{document}
 
Arpon Basu, School: AECS-4 , Mumbai-400094\\
 
Solution for Problem U373 \\

We define $a_{k}=1+\frac{1}{1+2+3+...+k+(k+1)}=1+\frac{2}{k+1}-\frac{2}{k+2}$ ,where  $1\leq k\leq n-1$.\\

Applying the AM-GM inequality to the numbers $a_{1}$,$a_{2}$,$a_{3}$,...,$a_{n-1}$,we get that:-\\
$(\frac{a_{1}+a_{2}+a_{3}+...+a_{n-1}}{n-1})^{n-1} > a_{1}a_{2}a_{3}...a_{n-1}$ (Note that a strict inequality holds because $a_{1}\neq a_{2}\neq a_{3}\neq ... \neq a_{n-1}$ for $n\geq 2$).\\
Now,
$(\frac{a_{1}+a_{2}+a_{3}+...+a_{n-1}}{n-1})^{n-1}=(\frac{(n-1)+2(\frac{1}{2}-\frac{1}{3}+\frac{1}{3}-\frac{1}{4}+...+\frac{1}{n}-\frac{1}{n+1})}{n-1})^{n-1}=(1+\frac{1}{2n+2})^{n-1}< (1+\frac{1}{n-1})^{n-1}$.\\
But,the upper bound of $(1+\frac{1}{n-1})^{n-1}$ as $n\rightarrow \infty $ is $e$,where $e$ is the base of natural logarithms.And since $e<3$,we get that:-\\
$a_{1}a_{2}a_{3}...a_{n-1}<(\frac{a_{1}+a_{2}+a_{3}+...+a_{n-1}}{n-1})^{n-1}<e<3$.\\ 

 
\end{document}